high2/Zeta.High.Interleave.fsti
@@ -37,6 +37,15 @@ let thread_store_post (#app #n:_) (tid: nat{tid < n}) (il: verifiable_log app n)
   = let vs = thread_state_post tid il i in
     vs.st
 
+val not_refs_implies_store_unchanged  (#app #n:_) (k:base_key) (t:nat{t < n})
+  (il: verifiable_log app n) (i:seq_index il)
+  : Lemma (ensures (let e = I.index il i in
+                    let st_pre = thread_store_pre t il i in
+                    let st_post = thread_store_post t il i in
+                    not (e `exp_refs_key` k) ==>
+                    store_contains st_pre k ==>
+                    (store_contains st_post k /\ st_pre k == st_post k)))
+
 val blum_evict_elem_props
   (#app #n:_)
   (il: verifiable_log app n)
@@ -90,11 +99,6 @@ let eac_state_of_key_post (#app #n:_) (k: base_key) (il: verifiable_log app n) (
   = let il' = prefix il (i+1) in
     eac_state_of_key k il'
 
-let eac_state_of_gkey (#app #n:_) (gk: key app) (il: verifiable_log app n)
-  : (eac_state app (to_base_key gk))
-  = let bk = to_base_key gk in
-    eac_state_of_key bk il
-
 (* is the key k in evicted state in *)
 let is_eac_state_evicted (#app #n:_) (k: base_key) (il: verifiable_log app n): bool
   = EACEvictedMerkle? (eac_state_of_key k il) ||
@@ -104,9 +108,19 @@ let is_eac_state_active (#app #n:_) (k: base_key) (il: verifiable_log app n)
   = let es = eac_state_of_key k il in
     es <> EACInit && es <> EACFail
 
-let is_eac_state_active_gk (#app #n:_) (gk: key app) (il: verifiable_log app n)
-  = let es = eac_state_of_gkey gk il in
-    es <> EACInit && es <> EACFail
+let is_eac_state_instore (#app #n:_) (k:base_key) (il: verifiable_log app n)
+  = let es = eac_state_of_key k il in
+    let open Zeta.BinTree in
+    k = Root && es = EACInit || EACInStore? es
+
+let eac_state_of_genkey (#app #n:_) (gk: key app) (il: verifiable_log app n)
+  : eac_state app (to_base_key gk)
+  = let k = to_base_key gk in
+    let es = eac_state_of_key k il in
+    if EAC.is_eac_state_active es then
+      if gk = to_gen_key es then es
+      else EACInit
+    else es
 
 val empty_implies_eac (#app #n:_) (il: verifiable_log app n)
   : Lemma (ensures (length il = 0 ==> is_eac il))
@@ -158,32 +172,28 @@ val eac_state_active_implies_prev_add (#app #n:_) (k: base_key) (il: eac_log app
 val eac_state_init_implies_no_key_refs (#app #n:_) (k: base_key) (il: eac_log app n)
   : Lemma (ensures (eac_state_of_key k il = EACInit ==> ~ (has_some_ref_to_key k il)))
 
-let to_gen_key (#app #n:_) (bk: base_key) (il: eac_log app n {is_eac_state_active bk il \/ is_merkle_key bk})
-  : gk:key app {to_base_key gk = bk}
-  = if is_merkle_key bk then IntK bk
-    else
-      let es = eac_state_of_key bk il in
-      match es with
-      | EACInStore _ gk _ -> gk
-      | EACEvictedBlum gk _ _ _ -> gk
-      | EACEvictedMerkle gk _ -> gk
-
 (* when the eac_state of k is instore, then k is in the store of a unique verifier thread *)
-val stored_tid (#app:_) (#n:nat) (k: base_key) (il: eac_log app n {EACInStore? (eac_state_of_key k il)})
+val stored_tid (#app:_) (#n:nat) (k: base_key) (il: eac_log app n {is_eac_state_instore k il})
   : tid:nat{tid < n /\
           (let st = thread_store tid il in
-           let gk = to_gen_key k il in
+           let es = eac_state_of_key k il in
+           let gk = to_gen_key es in
            store_contains st k /\ gk = stored_key st k)}
 
-val lemma_instore (#app #n:_) (bk: base_key{bk <> Zeta.BinTree.Root}) (il: eac_log app n)
-  : Lemma (ensures (exists_in_some_store bk il <==> EACInStore? (eac_state_of_key bk il)))
+val lemma_instore (#app #n:_) (bk: base_key) (il: eac_log app n)
+  : Lemma (ensures (exists_in_some_store bk il <==> is_eac_state_instore bk il))
 
 (* uniqueness: k is never in two stores *)
 val key_in_unique_store (#app #n:_) (k:base_key) (il: eac_log app n) (tid1 tid2: thread_id il)
   : Lemma (ensures (tid1 <> tid2 ==>
                     ~ (store_contains (thread_store tid1 il) k /\ store_contains (thread_store tid2 il) k)))
 
-let stored_value (#app #n:_) (gk: key app) (il: eac_log app n{EACInStore? (eac_state_of_gkey gk il)})
+let stored_value (#app #n:_)
+  (gk: key app)
+  (il: eac_log app n{let k = to_base_key gk in
+                     let es = eac_state_of_key k il in
+                     is_eac_state_instore k il /\
+                     to_gen_key es = gk})
   : value_t gk
   = let bk = to_base_key gk in
     let tid = stored_tid bk il in
@@ -226,17 +236,18 @@ let eac_state_evicted_value (#app #bk:_) (es: eac_state app bk {EAC.is_eac_state
 
 val eac_value_is_evicted_value (#app #n:_) (il: eac_log app n) (gk: key app):
   Lemma (requires (let bk = to_base_key gk in
+                   let es = eac_state_of_key bk il in
                    is_eac_state_evicted bk il /\
-                   gk = to_gen_key bk il))
+                   gk = to_gen_key es))
         (ensures (let bk = to_base_key gk in
                   let es = eac_state_of_key bk il in
                   eac_state_evicted_value es = eac_value gk il))
 
 val eac_value_init_state_is_init (#app #n:_) (il: eac_log app n) (gk: key app):
   Lemma (requires (let bk = to_base_key gk in
-                   let es = eac_state_of_key bk il in
-                   bk <> Zeta.BinTree.Root /\
-                   (es = EACInit \/ to_gen_key bk il <> gk)))
+                   let es = eac_state_of_genkey gk il in
+                   es = EACInit /\
+                   bk <> Zeta.BinTree.Root))
         (ensures (eac_value gk il = init_value gk))
 
 val eac_value_init
@@ -292,7 +303,7 @@ val root_never_added (#app #n:_) (il: verifiable_log app n) (i: seq_index il):
 
 val eac_app_state_value_is_stored_value (#app #n:_) (il: eac_log app n) (gk: key app)
   : Lemma (requires (let bk = to_base_key gk in
-                     let es = eac_state_of_key bk il in
+                     let es = eac_state_of_genkey gk il in
                      AppK? gk /\ EACInStore? es))
           (ensures (let bk = to_base_key gk in
                     let EACInStore _ gk' v = eac_state_of_key bk il in
